sha512_224sum.lean
@@ -1,0 +1,18 @@
+/-
+Copyright (c) 2026 Kim Morrison. All rights reserved.
+Released under Apache 2.0 license as described in the file LICENSE.
+Authors: Kim Morrison
+-/
+module
+
+import Crypto.CLI
+import Crypto.SHA2
+
+public section
+
+/-! # Command line interface for sha512_224sum -/
+
+open Crypto.CLI
+
+def main (args : List String) : IO UInt32 :=
+  runHashSumMain Crypto.Hash.Algorithm.sha512_224 args
